Dafny/examples/BasicBug/simpleBugProperties.i.dfy
@@ -47,31 +47,25 @@ module simpleBugProperties{
  lemma patchIssuccessful(s:state,patchBehaviors:seq<behavior>)
         requires ValidState(s);
         requires nonTrivialBehaviorPreconditionsPatch(s,patchBehaviors)
-        // ensures benignPatch(vulnBehaviors,patchBehaviors)
+        ensures successfulPatch(patchBehaviors)
     {    
         var result := LV("result");
          if (|patchBehaviors| == 0){
              assert forall p :: MiniSpec(p) ==> !(p in patchBehaviors);
          } else {
              assert |patchBehaviors| > 0;
+             assert forall q :: MiniSpec(q) ==> RemovedBehaviors(q);
              forall p | p in patchBehaviors
+                ensures !MiniSpec(p);
                 {  
                     var input :| BehaviorEvalsCode(codePatch(input),p) && |p| > 0 && validInput(p[0],input);
                     var b' := unwrapPatchBehaviors(s,input);
-                    // assert ValidOperand(last(p),result);
-                    // assert !RemovedBehaviorsUpdated(p);
-                    assert forall q :: MiniSpec(q) ==> RemovedBehaviors(q);
-                    assert forall q :: MiniSpec(q) ==> (exists s:state,result:operand :: (&& s in q
-                                                                                            && last(q) == s 
-                                                                                            && ValidState(s)
-                                                                                            && result.LV?
-                                                                                            && result.l in s.lvs
-                                                                                            && ValidOperand(s,result)
-                                                                                            && OperandContents(s,result).Int?
-                                                                                            && OperandContents(s,result).val == 0));
+                    behaviorThatEvalsSameCodeWithSameInitIsEqual(s,codePatch(input),b');
+                    assert !RemovedBehaviors(p);
+                    assert !MiniSpec(p);
                 }
                 
-                // assert forall p :: MiniSpec(p) ==> !(p in patchBehaviors);
+                assert forall p :: MiniSpec(p) ==> !(p in patchBehaviors);
              }
          }
     
