Dafny/examples/BasicBug/simpleBugSuccessfulLemmas.i.dfy
@@ -37,33 +37,25 @@ lemma possibleVulnOutputs(s:state, b:behavior)
      
     }
 
-    lemma possiblePatchOutputs(s:state, b:behavior) 
-        requires ValidState(s);
-        requires |b| > 0;
-        requires b[0] == s;
-        requires s.o.Nil?;
+    // lemma possiblePatchOutputs(s:state, b:behavior) 
+    //     requires ValidState(s);
+    //     requires |b| > 0;
+    //     requires b[0] == s;
+    //     requires s.o.Nil?;
 
-        ensures  forall input :: (validInput(s,input) && BehaviorEvalsCode(codeVuln(input),b)) 
-                                  ==> (behaviorOutput(b) == [Nil,Nil,Nil,Out((Int(1,IntType(1,false)))),Out((Int(1,IntType(1,false))))]);
-        // ensures  forall input :: (validInput(s,input) && OperandContents(s,input).val >= 2 && BehaviorEvalsCode(codeVuln(input),b)) 
-        //                           ==> (behaviorOutput(b) == [Nil,Nil,Nil,Out((Int(0,IntType(1,false)))),Out((Int(0,IntType(1,false))))]);
-    {
-        var inputWitness := D(Int(1,IntType(4,false)));
-        assert validInput(s,inputWitness);
-        forall input | validInput(s,input)  && BehaviorEvalsCode(codeVuln(input),b)
-            ensures (behaviorOutput(b) == [Nil,Nil,Nil,Out((Int(1,IntType(1,false)))),Out((Int(1,IntType(1,false))))]);
-        {
-            var input :| validInput(s,input) && BehaviorEvalsCode(codeVuln(input),b);
-            var b' := unwrapPatchBehaviors(s,input);
-        }
-        // forall input | validInput(s,input) && OperandContents(s,input).val >= 2 && BehaviorEvalsCode(codeVuln(input),b)
-        //     ensures (behaviorOutput(b) == [Nil,Nil,Nil,Out((Int(0,IntType(1,false)))),Out((Int(0,IntType(1,false))))]);
-        // {
-        //     var input :| validInput(s,input) && OperandContents(s,input).val >= 2 && BehaviorEvalsCode(codeVuln(input),b);
-        //     var b' := unwrapVulnBehaviors(s,input);
-        // }
+    //     ensures  forall input :: (validInput(s,input) && ValidBehaviorNonTrivial(b) && BehaviorEvalsCode(codePatch(input),b)) 
+    //                               ==> (behaviorOutput(b) == [Nil,Nil,Nil,Out((Int(1,IntType(1,false)))),Out((Int(1,IntType(1,false))))]);
+    // {
+    //     var inputWitness := D(Int(1,IntType(4,false)));
+    //     assert validInput(s,inputWitness);
+    //     forall input | validInput(s,input)  &&  ValidBehaviorNonTrivial(b) && BehaviorEvalsCode(codePatch(input),b)
+    //         ensures (behaviorOutput(b) == [Nil,Nil,Nil,Out((Int(1,IntType(1,false)))),Out((Int(1,IntType(1,false))))]);
+    //     {
+    //         var input :| validInput(s,input) && BehaviorEvalsCode(codePatch(input),b);
+    //         var b' := unwrapPatchBehaviors(s,input);
+    //     }
      
-    }
+    // }
 
 
 }
